RocqOfRust/ruint/fmt.v
@@ -666,7 +666,7 @@ Module fmt.
                                                                       M.borrow (|
                                                                         Pointer.Kind.Ref,
                                                                         M.deref (|
-                                                                          mk_byte_str_ref
+                                                                          M.mk_byte_str_ref
                                                                             8
                                                                             [
                                                                               211;
@@ -1296,7 +1296,7 @@ Module fmt.
                                                                       M.borrow (|
                                                                         Pointer.Kind.Ref,
                                                                         M.deref (|
-                                                                          mk_byte_str_ref
+                                                                          M.mk_byte_str_ref
                                                                             8
                                                                             [
                                                                               211;
@@ -1868,7 +1868,7 @@ Module fmt.
                                                                       M.borrow (|
                                                                         Pointer.Kind.Ref,
                                                                         M.deref (|
-                                                                          mk_byte_str_ref
+                                                                          M.mk_byte_str_ref
                                                                             8
                                                                             [
                                                                               211;
@@ -2440,7 +2440,7 @@ Module fmt.
                                                                       M.borrow (|
                                                                         Pointer.Kind.Ref,
                                                                         M.deref (|
-                                                                          mk_byte_str_ref
+                                                                          M.mk_byte_str_ref
                                                                             8
                                                                             [
                                                                               211;
@@ -3012,7 +3012,7 @@ Module fmt.
                                                                       M.borrow (|
                                                                         Pointer.Kind.Ref,
                                                                         M.deref (|
-                                                                          mk_byte_str_ref
+                                                                          M.mk_byte_str_ref
                                                                             8
                                                                             [
                                                                               211;
