RocqOfRust/ruint/string.v
@@ -803,7 +803,7 @@ Module string.
                               M.borrow (|
                                 Pointer.Kind.Ref,
                                 M.deref (|
-                                  mk_byte_str_ref
+                                  M.mk_byte_str_ref
                                     18
                                     [
                                       15;
@@ -912,7 +912,7 @@ Module string.
                               M.borrow (|
                                 Pointer.Kind.Ref,
                                 M.deref (|
-                                  mk_byte_str_ref
+                                  M.mk_byte_str_ref
                                     41
                                     [
                                       14;
